updates

Veritas.Record.fsti
@@ -1,6 +1,7 @@
 module Veritas.Record
 
 open FStar.BitVector
+open Veritas.BinTree
 open Veritas.Key
 
 (* data value - add a special value Null over an underlying type a*)
@@ -17,21 +18,26 @@ type hash_value = bv_t hash_size
 (* information about a desc stored in a merkle node *)
 type desc_hash = 
   | Empty: desc_hash
-  | Desc: k:merkle_key -> h:hash_value -> b:bool -> desc_hash
+  | Desc: k:key -> h:hash_value -> b:bool -> desc_hash
 
 (* merkle value: information about left and right descendants *)
 type merkle_value = 
-  | MValue: l:desc_hash -> r:desc_hash -> merkle_value
+  | MkValue: l:desc_hash -> r:desc_hash -> merkle_value
 
+let desc_hash_dir (v:merkle_value) (d:bin_tree_dir) = 
+  match d with
+  | Left -> MkValue?.l v
+  | Right -> MkValue?.r v
+  
 (* value - union type of merkle and data values *)
 type value = 
-  | Merkle: v:merkle_value -> value
-  | Data: v:data_value -> value
+  | MVal: v:merkle_value -> value
+  | DVal: v:data_value -> value
 
 (* check merkle/data consistency of k and v *)
 let is_value_of (k:key) (v:value) = 
-  if is_data_key k then Data? v
-  else Merkle? v
+  if is_data_key k then DVal? v
+  else MVal? v
 
 type value_type_of (k:key) = v:value{is_value_of k v}
 
@@ -39,3 +45,11 @@ type key_type_of (v:value) = k:key{is_value_of k v}
 
 (* record - key-value pair *)
 type record = key * value
+
+let init_value (k:key): v:value{is_value_of k v} = 
+  if is_data_key k then DVal Null
+  else MVal (MkValue Empty Empty)
+
+let to_merkle_value (v:value{MVal? v}) = MVal?.v v
+
+let to_data_value (v:value{DVal? v}) = DVal?.v v
