Veritas.Hash.fsti
@@ -1,0 +1,13 @@
+module Veritas.Hash
+
+open FStar.BitVector
+open Veritas.Record
+
+(* size of a hash value *)
+let hash_size = 256
+
+(* hash value *)
+type hash_value = bv_t hash_size
+
+(* hash function maps a merkle payload to a hash value *)
+val hashfn (v:value): Tot hash_value
