Veritas.Verifier.fst
@@ -1,7 +1,9 @@
 module Veritas.Verifier
 
 open FStar.Seq
+open Veritas.BinTree
 open Veritas.Key
+open Veritas.Hash
 open Veritas.Record
 open Veritas.SeqAux
 open Veritas.MultiSetHash
@@ -18,13 +20,13 @@ type vlog_entry =
   | Get: k:data_key -> v:data_value -> vlog_entry
   | Put: k:data_key -> v:data_value -> vlog_entry
   | AddM: r:record -> k':merkle_key -> vlog_entry
-  | EvictM: k:key -> k':merkle_key -> vlog_entry 
-  | AddB: r:record -> t:timestamp -> vlog_entry 
+  | EvictM: k:key -> k':merkle_key -> vlog_entry
+  | AddB: r:record -> t:timestamp -> vlog_entry
   | EvictB: k:key -> t:timestamp -> vlog_entry
   | EvictBM: k:key -> k':merkle_key -> vlog_entry
 
 (* verifier log entry (global)  *)
-type vlog_entry_g = 
+type vlog_entry_g =
   | Log: tid:nat -> e:vlog_entry -> vlog_entry_g
 
 (* verifier log *)
@@ -34,12 +36,12 @@ type vlog = seq vlog_entry_g
 type vl_index (l:vlog) = seq_index l
 
 (* for records in the store, how were they added? *)
-type add_method = 
+type add_method =
   | Merkle: add_method       (* AddM *)
   | Blum: add_method         (* AddB *)
 
 (* verifier store entry *)
-type vstore_entry (k:key) = 
+type vstore_entry (k:key) =
   | VStore: v:value_type_of k -> am: add_method -> vstore_entry k
 
 (* verifier store is a subset of (k,v) records *)
@@ -51,176 +53,179 @@ let store_contains (st:vstore) (k:key) = Some? (st k)
 
 (* lookup the value of a key in the store *)
 let stored_value (st:vstore) (k:key{store_contains st k}):
-  (value_type_of k) = 
+  (value_type_of k) =
   VStore?.v (Some?.v (st k))
 
 (* add method of a key in the store *)
-let add_method_of (st:vstore) (k:key{store_contains st k}): add_method = 
+let add_method_of (st:vstore) (k:key{store_contains st k}): add_method =
     VStore?.am (Some?.v (st k))
 
 (* update the store *)
-let update_store (st:vstore) 
+let update_store (st:vstore)
                  (k:key{store_contains st k})
                  (v:value_type_of k):
-  Tot (st':vstore {store_contains st' k /\ stored_value st' k = v}) = 
-  let am = add_method_of st k in                      
+  Tot (st':vstore {store_contains st' k /\ stored_value st' k = v}) =
+  let am = add_method_of st k in
   fun k' -> if k' = k then Some (VStore v am) else st k'
 
 (* add a new record to the store *)
 let add_to_store (st:vstore)
                  (k:key{not (store_contains st k)})
                  (v:value_type_of k)
-                 (am:add_method): 
+                 (am:add_method):
   (st':vstore{store_contains st' k /\ stored_value st' k = v}) =
   fun k' -> if k' = k then Some (VStore v am) else st k'
 
 (* evict a key from a store *)
 let evict_from_store (st:vstore)
-                     (k:key{store_contains st k}) = 
+                     (k:key{store_contains st k}) =
   fun k' -> if k' = k then None else st k'
 
 (* verifier thread local state  *)
-noeq type vtls = 
+noeq type vtls =
   | TLS: st:vstore -> clk:timestamp -> lk:key -> vtls
 
 (* per-epoch hash value *)
 type epoch_hash = nat -> ms_hash_value
 
 (* verifier global state *)
-noeq type vgs = 
-  | GS: hadd: epoch_hash -> 
+noeq type vgs =
+  | GS: hadd: epoch_hash ->
         hevict: epoch_hash ->
         ne:nat -> vgs
 
 (* verifier state aggregated across all verifier threads *)
-noeq type vstate (p:nat) = 
+noeq type vstate (p:nat) =
   | Failed: vstate p
   | Valid: tlss:seq vtls{length tlss = p} ->
            gs:vgs ->
            vstate p
 
-let thread_store (#p:nat) (i:nat{i < p}) (vs:vstate p{Valid? vs}): vstore = 
+(* get the store of a specified verifier thread *)
+let thread_store (#p:nat) (i:nat{i < p}) (vs:vstate p{Valid? vs}): vstore =
   let tlss = Valid?.tlss vs in
   let tls = index tlss i in
-  TLS?.st tls  
+  TLS?.st tls
 
-(* verifier read operation; return false on verification failure *)
-let vget (#p:nat) (i:nat{i < p}) 
+(* update the store of a specified verifier thread *)
+let update_thread_store (#p:nat)
+                        (i:nat{i < p})
+                        (vs:vstate p{Valid? vs})
+                        (st:vstore)
+                        : vstate p =
+  let tlss = Valid?.tlss vs in
+  let gs = Valid?.gs vs in
+  let tls = index tlss i in
+  match tls with
+  | TLS _ clk lk -> let tls' = TLS st clk lk in
+                    let tlss' = upd tlss i tls' in
+                    Valid tlss' gs
+
+(* verifier read operation *)
+let vget (#p:nat) (i:nat{i < p})
          (k:data_key) (v:data_value) (vs: vstate p{Valid? vs}): vstate p =
   let st = thread_store i vs in
-  
-  (* check store contains addr *)
+  (* check store contains key *)
   if not (store_contains st k) then Failed
-  
-  (* check stored payload is v *)
-  else if stored_value st k <> Data v then Failed 
-  
+  (* check stored value is v *)
+  else if to_data_value (stored_value st k) <> v then Failed
+  (* all checks pass - simply return state unchanged *)
   else vs
 
-(*
-(* verification write operation: return updated store on success; Null on failure *)
-let verifier_write (a:addr) (v:payload)
-                   (store: vstore): option vstore = 
-  (* merkle addr *)
-  let ma = addr_to_merkle_leaf a in  
-  (* check store contains addr *)
-  if not (store_contains store ma) then None
-  (* update the store *)
-  else Some (store_update store ma (MkLeaf v))
+(* verifier write operation *)
+let vwrite (#p:nat) (i:nat{i < p})
+           (k:data_key) (v:data_value) (vs: vstate p{Valid? vs}): vstate p =
+  let st = thread_store i vs in
+  (* check store contains key *)
+  if not (store_contains st k) then Failed
+  else update_thread_store i vs (update_store st k (DVal v))
 
-let is_empty_or_null (a:merkle_addr) (v:merkle_payload_of_addr a): Tot bool =
-  if is_merkle_leaf a then Null? (MkLeaf?.value v)
-  else Empty? (MkInternal?.left v) &&
-       Empty? (MkInternal?. right v)
-
-let update_desc_hash (v:merkle_payload_internal)
-                     (d:bin_tree_dir)
-                     (a:merkle_addr)
-                     (h:hash_value) =
+(* update merkle value *)
+let update_merkle_value (v:merkle_value)
+                        (d:bin_tree_dir)
+                        (k:key)
+                        (h:hash_value)
+                        (b:bool) =
   match v with
-  | MkInternal dhl dhr -> match d with 
-                         | Left -> MkInternal (Desc a h false) dhr
-                         | Right -> MkInternal dhl (Desc a h false)
+  | MkValue dhl dhr -> match d with
+                      | Left -> MkValue (Desc k h b) dhr
+                      | Right -> MkValue dhl (Desc k h b)
 
-let verifier_addm (s: vstore) 
-                  (a: merkle_addr)
-                  (v: merkle_payload)
-                  (a': merkle_addr): option vstore = 
-  (* check a is a proper desc of a' *)                  
-  if not (is_proper_desc a a') then None
-  (* check store contains a' *)
-  else if not (store_contains s a') then None
-  (* check store does not contain a *)
-  else if store_contains s a then None 
-  (* Check the payload type corresponds to leaf/internal ness of address a *)
-  else if not (is_payload_of_addr a v) then None
-  
-  else (
-    let v' = stored_payload s a' in
-    let d = desc_dir a a' in
-
-    lemma_proper_desc_depth_monotonic a a';
-    assert(not (is_merkle_leaf a'));
-    
-    let dh' = desc_hash_dir d v' in
+let vaddm (#p:nat) (i:nat{i < p})
+          (r:record)
+          (k':merkle_key)
+          (vs: vstate p{Valid? vs}): vstate p =
+  let st = thread_store i vs in
+  let (k,v) = r in
+  (* check k is a proper desc of k' *)
+  if not (is_proper_desc k k') then Failed
+  (* check store contains k' *)
+  else if not (store_contains st k') then Failed
+  (* check store does not contain k *)
+  else if store_contains st k then Failed
+  (* check that type of value is consistent with key *)
+  else if not (is_value_of k v) then Failed
+  else
+    let v' = to_merkle_value (stored_value st k') in
+    let d = desc_dir k k' in
+    let dh' = desc_hash_dir v' d in
     let h = hashfn v in
-
     match dh' with
-    | Empty -> if (is_empty_or_null a v) then 
-                 let v'_upd = update_desc_hash v' d a h in
-                 let s_upd = store_update s a' v'_upd in
-                 Some (store_add s_upd a v Merkle)
-               else None
-    | Desc a2 h2 b2 -> if a2 = a && h2 = h then Some (store_add s a v Merkle) 
-                       else if not (is_empty_or_null a v) then None                        
-                       else if not (is_proper_desc a2 a) then None
-                       else (
-                         lemma_proper_desc_depth_monotonic a2 a;
-                         assert(not (is_merkle_leaf a));
+    | Empty -> if v = init_value k then
+                 let v'_upd = update_merkle_value v' d k h false in
+                 let st_upd = update_store st k' (MVal v'_upd) in
+                 let st_upd2 = add_to_store st_upd k v Merkle in
+                 update_thread_store i vs st_upd2
+               else Failed
+    | Desc k2 h2 b2 -> if k2 = k then
+                         if h2 = h then
+                           update_thread_store i vs (add_to_store st k v Merkle)
+                         else Failed
+                       else if v <> init_value k then Failed
+                       else if not (is_proper_desc k2 k) then Failed
+                       else
+                         let d2 = desc_dir k2 k in
+                         let mv = to_merkle_value v in
+                         let mv_upd = update_merkle_value mv d2 k2 h2 b2 in
+                         let v'_upd = update_merkle_value v' d k h false in
+                         let st_upd = update_store st k'(MVal  v'_upd) in
+                         let st_upd2 = add_to_store st_upd k (MVal mv_upd) Merkle in
+                         update_thread_store i vs st_upd2
 
-                         let d2 = desc_dir a2 a in
-                         let v_upd = update_desc_hash v d2 a2 h2 in
-                         let v'_upd = update_desc_hash v' d a h in
-                         let s_upd = store_update s a' v'_upd in
-                         Some (store_add s_upd a v Merkle)
-                       )
-  )    
-
-let verifier_evictm (s: vstore)
-                    (a:merkle_addr)
-                    (a':merkle_addr): option vstore = 
+let vevictm (#p:nat) (i:nat{i < p})
+            (k:key)
+            (k':merkle_key)
+            (vs: vstate p{Valid? vs}): vstate p = 
+  let st = thread_store i vs in
   (* check store contains a and a' *)
-  if not (store_contains s a && store_contains s a') then None
-  else if is_merkle_root a then None
-  else if not (is_proper_desc a a') then None
-  else (
-    lemma_proper_desc_depth_monotonic a a';
-    assert(not (is_merkle_leaf a'));
-
-    let v' = stored_payload s a' in
-    let v = stored_payload s a in
-    let d = desc_dir a a' in
-    
-    lemma_proper_desc_depth_monotonic a a';
-    assert(not (is_merkle_leaf a'));
-    
-    let dh' = desc_hash_dir d v' in
+  if not (store_contains st k && store_contains st k') then Failed
+  else if not (is_proper_desc k k') then Failed
+  else
+    let v' = to_merkle_value (stored_value st k') in
+    let v = stored_value st k in
+    let d = desc_dir k k' in
+    let dh' = desc_hash_dir v' d in
     let h = hashfn v in
-
     match dh' with
-    | Empty -> None
-    | Desc a2 h2 b2 -> if a2 = a then 
-                         let v'_upd = update_desc_hash v' d a h in
-                         Some (store_evict (store_update s a' v'_upd) a)                       
-                       else None    
-  )
+    | Empty -> Failed
+    | Desc k2 h2 b2 -> if k2 = k then
+                         let v'_upd = update_merkle_value v' d k h b2 in
+                         let st_upd = evict_from_store (update_store st k' (MVal v'_upd)) k in
+                         update_thread_store i vs st_upd
+                       else Failed
+  
+(*
 
-let verifier_addb (#p:nat) 
-                  (i:nat {i < p}) 
+
+
+
+
+let verifier_addb (#p:nat)
+                  (i:nat {i < p})
                   (vs: vstate p{Valid? vs})
                   (a:merkle_addr)
                   (v:merkle_payload_of_addr a)
-                  (t:timestamp): (vstate p) = 
+                  (t:timestamp): (vstate p) =
   let tss = Valid?.tss vs in
   (* thread state *)
   let ts = index tss i in
@@ -235,46 +240,46 @@ let verifier_addb (#p:nat)
   if e < ne then Failed
 
   (* check that epoch e is at most 1 larger than ne *)
-  else if e + 1 > ne then Failed 
+  else if e + 1 > ne then Failed
 
   else (
     let epidx = e % 2 in
     admit()
   )
-    
-                  
+
+
 (* update the store of a specific thread *)
-let thread_update_store (#p:nat) (tid:nat {tid < p}) 
+let thread_update_store (#p:nat) (tid:nat {tid < p})
                         (vs:vstate p{Valid? vs})
-                        (store:vstore): vstate p = 
+                        (store:vstore): vstate p =
   let tss = Valid?.tss vs in
   let gs = Valid?.gs vs in
   let ts = index tss tid in
   match ts with
-  | VerifierThread _ clk lk -> 
+  | VerifierThread _ clk lk ->
     let ts_upd = VerifierThread store clk lk in
     let tss_upd = upd tss tid ts_upd in
     Valid tss_upd gs
 
-let verifier_step_thread (#p:nat) 
-                         (e:vlog_entry_thread) 
-                         (tid:nat {tid < p}) 
-                         (vs:vstate p{Valid? vs}): vstate p = 
+let verifier_step_thread (#p:nat)
+                         (e:vlog_entry_thread)
+                         (tid:nat {tid < p})
+                         (vs:vstate p{Valid? vs}): vstate p =
   let gs = Valid?.gs vs in
   let tss = Valid?.tss vs in
   let ts = index tss tid in
   let store = VerifierThread?.store ts in
   match e with
-  | MemoryOp o -> 
+  | MemoryOp o ->
     (
     match o with
-    | Read a v -> if verifier_read a v store       
+    | Read a v -> if verifier_read a v store
                   then vs
                   else Failed
     | Write a v -> let optStore = verifier_write a v store in
                    match optStore with
                    | None -> Failed
-                   | Some store' -> thread_update_store tid vs store'    
+                   | Some store' -> thread_update_store tid vs store'
     )
   | AddM a v a' -> let optStore = verifier_addm store a v a' in
                    (
@@ -290,18 +295,18 @@ let verifier_step_thread (#p:nat)
                    )
   | _ -> admit()
 
-let verifier_step (#p:nat) (e:vlog_entry) (vs:vstate p): vstate p = 
+let verifier_step (#p:nat) (e:vlog_entry) (vs:vstate p): vstate p =
   match vs with
   | Failed -> Failed              // propagate failures
-  | Valid ts gs -> 
+  | Valid ts gs ->
     match e with
     VLogEntry tid e' ->
-      if tid >= p then  Failed   // invalid thread id       
-      else verifier_step_thread e' tid vs        
+      if tid >= p then  Failed   // invalid thread id
+      else verifier_step_thread e' tid vs
 
 (* verify a log from a specified initial state *)
 let rec verifier_aux (#p:nat) (l:vlog) (vs:vstate p): Tot (vstate p)
-  (decreases (length l)) = 
+  (decreases (length l)) =
   let n = length l in
   if n = 0 then vs
   else
@@ -313,6 +318,6 @@ let rec verifier_aux (#p:nat) (l:vlog) (vs:vstate p): Tot (vstate p)
 (* initialize verifier state *)
 let init_vstate (p:nat): vstate p = admit()
 
-let verifier (p:nat) (l:vlog): Tot (vstate p) = 
+let verifier (p:nat) (l:vlog): Tot (vstate p) =
   verifier_aux l (init_vstate p)
 *)
